theories/util/point_free.v
@@ -3,9 +3,16 @@ From stdpp Require Import prelude.
 
 (** * Utility for Point-Free Style *)
 
+Lemma compose_assoc {A B C D} (f: A → B) (g: B → C) (h: C → D) :
+h ∘ (g ∘ f) = (h ∘ g) ∘ f.
+Proof. by rewrite /compose. Qed.
+
+Infix "=ₚ" := (pointwise_relation _ (=)) (at level 70).
+Notation "(=ₚ)" := (pointwise_relation _ (=)) (only parsing).
+
 Definition s_comb {A B C} (f: A → B → C) (g: A → B) x := (f x) (g x).
-Global Infix "⊛" := (s_comb) (left associativity, at level 50).
+Infix "⊛" := s_comb (left associativity, at level 50).
 
 Lemma surjective_pairing_fun {A B C} (f: A → B * C) :
-  pointwise_relation _ (=) f (pair ∘ (fst ∘ f) ⊛ (snd ∘ f)).
+  f =ₚ (pair ∘ (fst ∘ f) ⊛ (snd ∘ f)).
 Proof. move=> ?. by rewrite /s_comb /compose -surjective_pairing. Qed.
