theories/util/types.v
@@ -1,5 +1,6 @@
 From stdpp Require Import prelude.
-From iris.algebra Require Import ofe.
+From iris.algebra Require Import monoid ofe.
+From iris.base_logic Require Export iprop.
 
 (** * List of Types *)
 (** We avoid using [list Type] because that can cause universe inconsistency *)
@@ -7,21 +8,20 @@ From iris.algebra Require Import ofe.
 Inductive Types := tnil: Types | tcons: Type → Types → Types.
 Implicit Type As: Types.
 
-Notation "^[ ]" := (tnil) (at level 5, format "^[ ]").
-Infix "^::" := (tcons) (at level 60, right associativity).
+Notation "^[ ]" := tnil (at level 5, format "^[ ]").
+Infix "^::" := tcons (at level 60, right associativity).
 Notation "^[ A ; .. ; B ]" := (A ^:: .. (B ^:: ^[]) ..)
   (at level 5, format "^[ A ;  .. ;  B ]").
 
-Fixpoint app_Types As Bs :=
-  match As with ^[] => Bs | A ^:: As' => A ^:: app_Types As' Bs end.
-Infix "^++" := (app_Types) (at level 60, right associativity).
+Fixpoint tapp As Bs :=
+  match As with ^[] => Bs | A ^:: As' => A ^:: tapp As' Bs end.
+Infix "^++" := tapp (at level 60, right associativity).
 
 (** * Heterogeneous List *)
 
 Inductive hlist F : Types → Type :=
 | hnil: hlist F ^[]
 | hcons {A As} : F A → hlist F As → hlist F (A ^:: As).
-
 Notation "+[ ]" := (hnil _) (at level 1, format "+[ ]").
 Notation "+[ ]@{ F }" := (hnil F) (at level 1, only parsing).
 Infix "+::" := (hcons _) (at level 60, right associativity).
@@ -34,15 +34,15 @@ Notation "+[ x ; .. ; z ]@{ F }" := (x +:: .. (z +:: +[]@{F}) ..)
 Fixpoint happ {F As Bs} (xl: hlist F As) (yl: hlist F Bs)
   : hlist F (As ^++ Bs) :=
   match xl with +[] => yl | x +:: xl' => x +:: happ xl' yl end.
-Infix "+++" := (happ) (at level 60, right associativity).
+Infix "+++" := happ (at level 60, right associativity).
 
 Fixpoint hmap {F B As} (f: ∀A, F A → B) (xl: hlist F As) : list B :=
   match xl with +[] => [] | x +:: xl' => f _ x :: hmap f xl' end.
-Infix "+<$>" := (hmap) (at level 61, left associativity).
+Infix "+<$>" := hmap (at level 61, left associativity).
 
 Fixpoint hhmap {F G As} (f: ∀A, F A → G A) (xl: hlist F As) : hlist G As :=
   match xl with +[] => +[] | x +:: xl' => f _ x +:: hhmap f xl' end.
-Infix "+<$>+" := (hhmap) (at level 61, left associativity).
+Infix "+<$>+" := hhmap (at level 61, left associativity).
 
 Inductive HForall {F} (Φ: ∀A, F A → Prop) : ∀{As: Types}, hlist F As → Prop :=
 | HForall_nil: HForall Φ +[]
@@ -50,10 +50,35 @@ Inductive HForall {F} (Φ: ∀A, F A → Prop) : ∀{As: Types}, hlist F As → 
     Φ _ x → HForall Φ xl → HForall Φ (x +:: xl).
 
 Inductive HForall2 {F G} (Φ: ∀A, F A → G A → Prop)
-  : ∀{As: Types}, hlist F As → hlist G As → Prop :=
+  : ∀{As}, hlist F As → hlist G As → Prop :=
 | HForall2_nil: HForall2 Φ +[] +[]
 | HForall2_cons {A As} (x: _ A) (y: _ A) (xl: _ As) (yl: _ As) :
     Φ _ x y → HForall2 Φ xl yl → HForall2 Φ (x +:: xl) (y +:: yl).
+
+Fixpoint big_sepHL {Σ F As} (Φ: ∀A, F A → iProp Σ) (xl: hlist F As) : iProp Σ :=
+  match xl with +[] => True | x +:: xl' => Φ _ x ∗ big_sepHL Φ xl' end.
+Notation "'[∗' 'hlist]' x ∈ xl , P" := (big_sepHL (λ _ x, P) xl)
+  (at level 200, xl at level 10, x at level 1, right associativity,
+   format "[∗  hlist]  x  ∈  xl ,  P") : bi_scope.
+
+Inductive hlist2 F : Types → Types → Type :=
+| hnil2: hlist2 F ^[] ^[]
+| hcons2 {A B As Bs} : F A B → hlist2 F As Bs → hlist2 F (A ^:: As) (B ^:: Bs).
+Notation "+2[ ]" := (hnil2 _) (at level 1, format "+2[ ]").
+Notation "+2[ ]@{ F }" := (hnil2 F) (at level 1, only parsing).
+Infix "+2::" := (hcons2 _) (at level 60, right associativity).
+Infix "+2::@{ F }" := (hcons2 F) (at level 60, right associativity, only parsing).
+Notation "+2[ x ; .. ; z ]" := (x +2:: .. (z +2:: +2[]) ..)
+  (at level 1, format "+2[ x ;  .. ;  z ]").
+Notation "+2[ x ; .. ; z ]@{ F }" := (x +2:: .. (z +2:: +2[]@{F}) ..)
+  (at level 1, only parsing).
+
+Inductive HForall3 {F G H} (Φ: ∀A B, F A B → G A → H B → Prop)
+  : ∀{As Bs}, hlist2 F As Bs → hlist G As → hlist H Bs → Prop :=
+| HForall3_nil: HForall3 Φ +2[] +[] +[]
+| HForall3_cons {A B As Bs} (x: _ A B) y z (xl: _ As Bs) yl zl :
+    Φ _ _ x y z → HForall3 Φ xl yl zl →
+    HForall3 Φ (x +2:: xl) (y +:: yl) (z +:: zl).
 
 Section setoid.
 Context {F: Type → Type} `{∀A, Equiv (F A)}.
@@ -78,10 +103,10 @@ Inductive nil_unit := nil_tt: nil_unit.
 Inductive cons_prod A B := cons_pair: A → B → cons_prod A B.
 Arguments cons_pair {_ _} _ _.
 
-Notation ":1" := (nil_unit) (at level 1) : type_scope.
-Infix ":*" := (cons_prod) (at level 60, right associativity) : type_scope.
-Notation "-[ ]" := (nil_tt) (at level 1, format "-[ ]").
-Infix "-::" := (cons_pair) (at level 60, right associativity).
+Notation ":1" := nil_unit (at level 1) : type_scope.
+Infix ":*" := cons_prod (at level 60, right associativity) : type_scope.
+Notation "-[ ]" := nil_tt (at level 1, format "-[ ]").
+Infix "-::" := cons_pair (at level 60, right associativity).
 Notation "-[ a ; .. ; z ]" := (a -:: .. (z -:: -[]) ..)
   (at level 1, format "-[ a ;  .. ;  z ]").
 
@@ -90,4 +115,4 @@ Fixpoint flist F As : Type :=
 Fixpoint app_flist {F As Bs} (xl: flist F As) (yl: flist F Bs)
   : flist F (As ^++ Bs) := match As, xl with
   | ^[], -[] => yl | A ^:: As', x -:: xl' => x -:: app_flist xl' yl end.
-Infix "-++" := (app_flist) (at level 60, right associativity).
+Infix "-++" := app_flist (at level 60, right associativity).
